StateModel

Impl/CommitterModel.i.dfy
@@ -13,7 +13,14 @@ module CommitterModel {
   import opened Options
   import opened NativeTypes
 
+  datatype Status =
+    | StatusLoadingSuperblock
+    | StatusLoadingOther
+    | StatusReady
+
   datatype CommitterModel = CommitterModel(
+    status: Status,
+
     journalist: JournalistModel.JournalistModel,
     frozenLoc: Option<Location>,
     isFrozen: bool,
@@ -21,13 +28,68 @@ module CommitterModel {
     frozenJournalPosition: uint64,
     superblockWrite: Option<JC.ReqId>,
 
-    outstandingJournalWrites: seq<JC.ReqId>,
+    outstandingJournalWrites: set<JC.ReqId>,
 
     superblock: Superblock,
-    newSuperblock: Superblock,
+    newSuperblock: Option<Superblock>,
     whichSuperblock: uint64,
     commitStatus: JC.CommitStatus,
 
+    journalFrontRead: Option<JC.ReqId>,
+    journalBackRead: Option<JC.ReqId>,
+    superblock1Read: Option<JC.ReqId>,
+    superblock2Read: Option<JC.ReqId>,
+    superblock1: JC.SuperblockReadResult,
+    superblock2: JC.SuperblockReadResult,
+
     syncReqs: MutableMapModel.LinearHashMap<JC.SyncReqStatus>
   )
+
+  predicate WF(cm: CommitterModel)
+  {
+    && MutableMapModel.Inv(cm.syncReqs)
+    && JournalistModel.Inv(cm.journalist)
+  }
+
+  function I(cm: CommitterModel) : JC.Variables
+  requires WF(cm)
+  {
+    match cm.status {
+      case StatusLoadingSuperblock =>
+        JC.LoadingSuperblock(
+          cm.superblock1Read,
+          cm.superblock2Read,
+          cm.superblock1,
+          cm.superblock2,
+          cm.syncReqs.contents
+        )
+      case StatusLoadingOther =>
+        JC.LoadingOther(
+          cm.superblock,
+          cm.whichSuperblock as int,
+          cm.journalFrontRead,
+          cm.journalBackRead,
+          JournalistModel.I(cm.journalist).journalFront,
+          JournalistModel.I(cm.journalist).journalBack,
+          cm.syncReqs.contents
+        )
+      case StatusReady =>
+        JC.Ready(
+          cm.frozenLoc,
+          cm.isFrozen,
+          cm.frozenJournalPosition as int,
+          cm.superblockWrite,
+          JournalistModel.I(cm.journalist).inMemoryJournalFrozen,
+          JournalistModel.I(cm.journalist).inMemoryJournal,
+          cm.outstandingJournalWrites,
+          JournalistModel.I(cm.journalist).writtenJournalLen,
+          JournalistModel.I(cm.journalist).replayJournal,
+          cm.superblock,
+          cm.whichSuperblock as int,
+          cm.commitStatus,
+          cm.newSuperblock,
+          cm.syncReqs.contents
+        )
+    }
+  }
 }
